trial at delete

BSTExtra.v
@@ -2,6 +2,8 @@ Require Import BstProject.BST.
 Require Import BstProject.project_lib.
 Require Import Coq.Bool.Bool.
 Require Import Coq.Arith.Arith.
+Require Import Lia.
+Transparent BST.insert.
 
 (* bst to list *)
 Fixpoint bst_to_list (bst: tree) : list nat :=
@@ -10,20 +12,16 @@ Fixpoint bst_to_list (bst: tree) : list nat :=
   | node l v r => bst_to_list l ++ [v] ++ bst_to_list r
 end.
 
+
+
 Definition list_to_bst (lst: list nat) : tree :=
   fold_left(fun acc elem => insert elem acc) lst leaf.
 
 Example bst_lst : bst_to_list tree1 = [2;5;7;10;12;16;17].
 Proof. unfold bst_to_list. reflexivity. Qed.
 
-(* node (node (node leaf 2 leaf) 5 (node leaf 7 leaf))
-10 (* root *)
-(node (node leaf 12 leaf) 16 (node leaf 17 leaf)). *)
-(* [12; 17; 16; 2; 7; 5; 10] *)
-
 Example lst_bst : list_to_bst [10;5;7;2;16;17;12] =  tree1.
-Proof. unfold list_to_bst. simpl. Admitted.
-  (* reflexivity.  *)
+Proof. unfold list_to_bst. reflexivity. Qed.
 
 (*Useful Theorems *)
 (* Theorem bst_list_sorted : list -> bst -> list - skulle give sorted list ud
@@ -35,14 +33,11 @@ bst_to_list t1 = bst_to_list t2
 
 (* Exercise 3.10*)
 (* Find smallest value in right subtree -> expects to get right subtree *)
-Fixpoint successor (t:tree) : tree :=
-  match t with
-  | node l v r => 
-    match l with
-    | leaf => t
-    | _ => successor l
-    end
-  | leaf => t
+Fixpoint successor (t:tree) : option nat :=
+  match t with 
+  | leaf => None
+  | node leaf v _ => Some v 
+  | node l _ _  => successor l
 end.
 
 Fixpoint delete (x : nat) (t : tree) : tree :=
@@ -55,10 +50,9 @@ Fixpoint delete (x : nat) (t : tree) : tree :=
       | leaf, _ => r
       | _, leaf => l
       | _,_ => 
-        let succ := successor r in
-        match succ with
-        | node l' v' r' => node l v' (delete v' r)
-        | leaf => leaf (*Impossible -> TODO: make option (None)*)
+        match successor r with
+        | Some v' => node l v' (delete v' r)
+        | None => leaf (*Impossible -> TODO: make option (None)*)
         end
       end
     else if x <? v then
@@ -85,24 +79,241 @@ Example delete_root : delete 10 tree1 =
   (node leaf 16 (node leaf 17 leaf)).
 Proof. unfold delete. reflexivity. Qed.
 
-(* TODO: Lemma delete_sorted  *)
+(* Lemmas to help prove sorted*)
+
+
+(* If successor exists, it satisfies smaller property *)
+Lemma successor_smaller : forall n t v,
+  smaller n t -> successor t = Some v -> n < v.
+Proof.
+  induction t; intros. simpl in H0.
+  - discriminate.
+  - inversion H; subst. destruct t1; simpl in *.
+    + injection H0 as H0; subst. assumption.
+    + eapply IHt1; eauto.
+Qed.
+
+Lemma successor_unfold :
+  forall r1 n1 r2 v,
+    successor (node r1 n1 r2) = Some v ->
+    match r1 with
+    | leaf => Some n1
+    | node _ _ _ => successor r1
+    end = Some v.
+Proof.
+  intros r1 n1 r2 v H.
+  simpl in H.
+  destruct r1; simpl in *; auto.
+Qed.
+
+
+(* Successor is the minimum in the right subtree, so it's >= root in BST *)
+Lemma successor_greater : forall n t v,
+  greater n t -> successor t = Some v -> n > v.
+Proof.
+  induction t; intros; simpl in *.
+  - discriminate.
+  - inversion H; subst. destruct t1; simpl in *.
+    + injection H0 as H0; subst. assumption.
+    + eapply IHt1; eauto.
+Qed.
+
+(* In a sorted BST, the successor from right subtree is greater than all left *)
+Lemma successor_greater_than_left : forall l v r succ_v,
+  sorted (node l v r) ->
+  successor r = Some succ_v ->
+  greater succ_v l.
+Proof.
+  intros. inversion H; subst.
+  assert (v < succ_v).
+  { eapply successor_smaller; eauto. }
+  induction l.
+  - constructor.
+  - inversion H4; subst. constructor.
+    +  lia.
+    + apply IHl1; eauto.
+      * constructor; try assumption.
+       -- inversion H5; inversion H6; subst; assumption.
+      * inversion H5; inversion H6; subst; assumption.
+    + apply IHl2; eauto.
+      * constructor; try assumption.
+       -- inversion H5; inversion H6; subst; assumption.
+      * inversion H5; inversion H6; subst; assumption.
+Qed.
+
+
+Lemma smaller_delete_any : forall n x t,
+  smaller n t -> smaller n (delete x t).
+Proof.
+  induction t as [| l IHl v r IHr]; intros; simpl.
+  - exact H.
+  - inversion H; subst; clear H.
+    destruct (v =? x) eqn:Heq.
+    + destruct l.
+      * exact H6.
+      * destruct r.
+        -- exact H5.
+        -- simpl. destruct (successor (node r1 n1 r2)) eqn:Hsucc.
+           ++ pose proof (successor_unfold r1 n1 r2 n2 Hsucc) as Hunf.
+              rewrite Hunf. constructor.
+              ** eapply successor_smaller; eauto.
+              ** exact H5.
+              ** admit. 
+              (* apply IHr. exact H6. *)
+           ++ simpl in Hsucc. admit. 
+           (* destruct r1; discriminate. *)
+    + destruct (x <? v) eqn:Hlt.
+      * constructor; try assumption. apply IHl; assumption.
+      * constructor; try assumption. apply IHr; assumption.
+Admitted.
+
+(* In a sorted BST, successor from right is smaller than all right after deletion *)
+Lemma successor_smaller_than_right : 
+  forall r succ_v,
+    sorted r ->
+    successor r = Some succ_v ->
+    smaller succ_v (delete succ_v r).
+Proof.
+  induction r; intros; simpl in *.
+  - discriminate.
+  - destruct r1; simpl in *.
+    + (* Base case: successor is the root *)
+      injection H0 as H0; subst.
+      simpl. rewrite Nat.eqb_refl. 
+      inversion H; subst. eauto.
+    + (* Recursive case *)
+      inversion H; subst.
+      destruct (n =? succ_v) eqn:Heq.
+      * (* n = succ_v, impossible since successor is in left *)
+        simpl in H0. destruct r1_1.
+        -- (* Left subtree is leaf, so successor is n *)
+           injection H0 as H0; subst.
+           simpl. 
+           inversion H; subst. destruct r2.
+           ++ constructor.
+              ** exfalso. inversion H; subst. rewrite Nat.eqb_eq in Heq. subst. inversion H4; subst. lia.
+              ** eauto.
+              ** inversion H6. subst. eauto.
+          ++ destruct (successor (node r2_1 n0 r2_2)) eqn:Hsucc2; try eauto.
+              ** constructor.
+                --- (* Left subtree has successor *)
+                rewrite Nat.eqb_eq in Heq. subst. eapply successor_smaller; try eauto.
+                --- constructor; try (inversion H6; subst; eauto).
+                  *** exfalso. inversion H; subst. rewrite Nat.eqb_eq in Heq. subst. inversion H4; subst. lia.
+                --- rewrite Nat.eqb_eq in Heq. subst. apply smaller_delete_any. eauto.
+          -- (* Left subtree is not leaf, contradicts n = succ_v *)
+           simpl in H0. 
+           admit.
+      * destruct (succ_v <? n) eqn:Hlt.
+        -- (* Delete from left *)
+           simpl. constructor.
+           ++ eapply successor_smaller; eauto. admit.
+           ++ apply IHr1; assumption.
+           ++ eauto. admit.
+        -- (* succ_v >= n, but we know succ_v < n from BST property *)   
+        (* assert (succ_v < n) by 
+           (eapply successor_smaller; eauto).
+           rewrite Nat.ltb_lt in Hlt. lia. *)
+Admitted.
+
+Lemma successor_greater_root :
+  forall r1 n1 r2 v,
+    successor (node r1 n1 r2) = Some v ->
+    n1 >= v.
+Proof.
+  intros r1 n1 r2 v H.
+  simpl in H. 
+  destruct r1; simpl in *.
+  - inversion H. subst. lia.
+  - admit.
+Admitted.
+
+Lemma greater_delete : forall n x t,
+  greater n t -> greater n (delete x t).
+Proof.
+  induction t as [| l IHl v r IHr]; intros; simpl.
+  - exact H.
+  - inversion H; subst; clear H.
+    destruct (v =? x) eqn:Heq.
+    + destruct l.
+      * exact H6.
+      * destruct r.
+        -- exact H5.
+        -- simpl. destruct (successor (node r1 n1 r2)) eqn:Hsucc.
+           ++ pose proof (successor_unfold r1 n1 r2 n2 Hsucc) as Hunf.
+              rewrite Hunf. constructor.
+              ** eapply successor_greater; eauto.
+              ** exact H5.
+              ** admit. 
+              (* apply IHr. exact H6. *)
+           ++ simpl in Hsucc. 
+           admit. 
+           (* destruct r1; discriminate. *)
+    + destruct (x <? v) eqn:Hlt.
+      * constructor; try assumption. apply IHl; assumption.
+      * constructor; try assumption. apply IHr; assumption.
+Admitted.
+
+Hint Resolve successor_smaller : core.
+Hint Resolve successor_unfold : core.
+Hint Resolve successor_greater : core.
+Hint Resolve successor_greater_than_left : core.
+Hint Resolve smaller_delete_any : core.
+Hint Resolve successor_smaller_than_right : core.
+Hint Resolve successor_greater_root : core.
+Hint Resolve greater_delete : core.
+
 Lemma delete_sorted :
   forall t x, sorted t -> sorted (delete x t).
 Proof.
    induction t; simpl; intros.
-  - constructor; easy.
-  - inversion H; subst.
-Qed.
-  
+  - assumption.
+  - inversion H; subst. destruct (n=?x) eqn:Heq.
+    + (* Deleting the root *)
+      destruct t1.
+      * assumption.
+      * destruct t2.
+        -- assumption.
+        -- (* Two-child case *)
+           destruct (successor (node t2_1 n1 t2_2)) eqn:Hsucc.
+           ++ simpl in Hsucc. destruct t2_1; try discriminate.
+              ** (* Right child has no left subtree *)
+                 injection Hsucc as Hsucc; subst.
+                 simpl. constructor.
+                 --- apply successor_greater_than_left with (v := n) (r := node leaf n2 t2_2); try eauto.
+                 --- admit.
+                  (* apply smaller_delete_any. 
+                     apply successor_smaller_than_right with (r := node leaf n1 t2_2); assumption. *)
+                 --- assumption.
+                 --- apply IHt2. assumption.
+              ** (* Right child has left subtree *)
+                 constructor.
+                 --- apply successor_greater_than_left with (v := n) (r := node (node t2_1_1 n2 t2_1_2) n1 t2_2); try eauto.
+                 (* apply successor_greater_than_left with (r := node (node t2_1_1 n2 t2_1_2) n1 t2_2); assumption. *)
+                 --- apply smaller_delete_any. admit.
+                     (* apply successor_smaller_than_right with (r := node (node t2_1_1 n2 t2_1_2) n1 t2_2); assumption. *)
+                 --- assumption.
+                 --- apply IHt2. assumption.
+           ++ simpl in Hsucc. admit.
+    + (* Not deleting root, recurse *)
+      destruct (x <? n) eqn:Hlt.
+      * constructor; try eauto.
+        -- apply greater_delete. assumption.
+      * constructor; try eauto.
+        -- apply smaller_delete_any. assumption.
+Admitted.
+
+
 Lemma delete_correct :
 forall t x,
     sorted t ->
     elem_of x t = true -> 
     (elem_of x (delete x t)) = false.
 Proof.
-  induction t; simpl; intros.
+  intros. 
+  induction t. simpl; intros.
   - admit.
   - inversion H. 
-Qed.
+Admitted.
   
 
