BSTInsert.v
@@ -1,20 +1,311 @@
 Require Import BstProject.BST.
 Require Import BstProject.project_lib.
 Require Import Coq.Bool.Bool.
-Require Import Coq.Init.Nat.
+Require Import Coq.Arith.Arith.
+Require Import Lia.
+Transparent BST.insert.
 
-(* Exercise 3.8  *)
-Lemma insert_sorted :
-  forall t x, sorted t -> sorted (insert x t).
+(* bst to list *)
+Fixpoint bst_to_list (bst: tree) : list nat :=
+  match bst with
+  | leaf => []
+  | node l v r => bst_to_list l ++ [v] ++ bst_to_list r
+end.
+
+
+
+Definition list_to_bst (lst: list nat) : tree :=
+  fold_left(fun acc elem => insert elem acc) lst leaf.
+
+Example bst_lst : bst_to_list tree1 = [2;5;7;10;12;16;17].
+Proof. unfold bst_to_list. reflexivity. Qed.
+
+Example lst_bst : list_to_bst [10;5;7;2;16;17;12] =  tree1.
+Proof. unfold list_to_bst. reflexivity. Qed.
+
+(*Useful Theorems *)
+(* Theorem bst_list_sorted : list -> bst -> list - skulle give sorted list ud
+forall t1 t2, 
+bst_to_list t1 = bst_to_list t2
+*)
+
+(* Size of list equals size of tree *)
+
+(* Exercise 3.10*)
+(* Find smallest value in right subtree -> expects to get right subtree *)
+Fixpoint successor (t:tree) : option nat :=
+  match t with 
+  | leaf => None
+  | node leaf v _ => Some v 
+  | node l _ _  => successor l
+end.
+
+Fixpoint delete (x : nat) (t : tree) : tree :=
+  match t with
+  | leaf => leaf
+  | node l v r =>
+    if v =? x then
+      (*delete happens here*)
+      match l,r with
+      | leaf, _ => r
+      | _, leaf => l
+      | _,_ => 
+        match successor r with
+        | Some v' => node l v' (delete v' r)
+        | None => leaf (*Impossible -> TODO: make option (None)*)
+        end
+      end
+    else if x <? v then
+      node (delete x l) v r
+    else
+      node l v (delete x r)
+end.
+
+Example delete_one_child : delete 5 (node (node (node leaf 2 leaf ) 5 leaf) 10 leaf) = node (node leaf 2 leaf ) 10 leaf.
+Proof. unfold delete. reflexivity. Qed.
+
+Example delete_no_children : delete 2 (node (node (node leaf 2 leaf ) 5 leaf) 10 leaf) = node (node leaf 5 leaf ) 10 leaf.
+Proof. unfold delete. reflexivity. Qed.
+
+Example delete_two_children : delete 5 tree1 =   
+      node (node (node leaf 2 leaf) 7 leaf)
+       10 (* root *)
+      (node (node leaf 12 leaf) 16 (node leaf 17 leaf)).
+Proof. unfold delete. simpl. reflexivity. Qed.
+
+Example delete_root : delete 10 tree1 =
+  node (node (node leaf 2 leaf) 5 (node leaf 7 leaf))
+  12 (* new root *)
+  (node leaf 16 (node leaf 17 leaf)).
+Proof. unfold delete. reflexivity. Qed.
+
+(* Lemmas to help prove sorted*)
+
+(* Minimum value property in right subtree *)
+Lemma successor_all_right :
+  forall r m,
+    sorted r ->
+    successor r = Some m ->
+    smaller m r.
 Proof.
-  (*TODO: prove insert_sorted*)
- Admitted.
-(* Exercise 3.9 *)
-Lemma insert_correct :
-  forall t x y,
-    sorted t ->
-    elem_of y (insert x t)
-    = orb (elem_of y t) (Nat.eqb x y).
+  induction r; intros m Hsrt Hsucc; simpl in *; try discriminate.
+  destruct r1; inversion Hsrt; subst.
+  - (* left = leaf, root is successor *)
+    (* inversion Hsucc; subst m. constructor. 
+    try eauto. try lia. admit. *)
+     (* successor in left subtree *)
+    injection Hsucc as <-. constructor; try eauto.
+    + contradiction. exfalso. admit.
+    (* + assumption. *)
+  - (* successor in left subtree *)
+    admit. 
+Admitted.
+
+Lemma delete_unfold_node (x v : nat) (l r : tree) :
+  delete x (node l v r) =
+    if v =? x then
+      match l, r with
+      | leaf, _ => r
+      | _, leaf => l
+      | _, _ =>
+          match successor r with
+          | Some v' => node l v' (delete v' r)
+          | None => leaf
+          end
+      end
+    else if x <? v then node (delete x l) v r
+    else node l v (delete x r).
+Proof. reflexivity. Qed.
+
+(* Successor greater than all left subtree of original node *)
+Lemma successor_greater_than_left :
+  forall l v r m,
+    sorted (node l v r) ->
+    successor r = Some m ->
+    greater m l.
 Proof.
-  (*TODO: prove insert_correct*)
+  intros l v r m Hsrt Hsucc.
+  inversion Hsrt; subst.
+  (* Get smaller m r from successor_all_right *)
+  assert (Hsm_m_r : smaller m r) by (eapply successor_all_right; eauto).
+  (* smaller v r gives v < all elems of r, successor_smaller gives v < m *)
+  assert (v < m) by (admit).
+  (* Use greater v l and transitivity: for any x in l, x < v < m *)
+  revert H3. (* H3 is greater v l *)
+  induction l; intros Hgl; constructor.
+  - inversion Hgl; subst; admit.
+  - inversion Hgl; subst.
+    + admit.
+    + apply IHl1; admit.
   Admitted.
+
+
+(* Delete preserves 'smaller' when we delete ANY x (except root collapse case is handled by pattern) *)
+Lemma smaller_delete_any :
+  forall n x t,
+    smaller n t ->
+    smaller n (delete x t).
+Proof.
+  induction t; intros; simpl.
+  - assumption.
+  - inversion H; subst.
+    destruct (n0 =? x) eqn:Heq.
+    + (* deleting root *)
+      destruct t1, t2; simpl; try assumption.
+      (* two-child case: rebuilding root with successor; need smaller n new_tree *)
+      all: destruct (successor (node t2_1 n0 t2_2)) eqn:Hsucc; try assumption.
+      * (* Successor found *)
+        admit.
+      * (* No successor: impossible since right has at least root *)
+        simpl in Hsucc. admit.
+    + destruct (x <? n0) eqn:Hlt.
+      * constructor; try assumption; apply IHt1; assumption.
+      * constructor; try assumption; apply IHt2; assumption.
+Admitted.
+
+(* Helper: if n > all elements of t, then n > successor of t *)
+Lemma greater_than_successor :
+  forall n t m,
+    greater n t ->
+    successor t = Some m ->
+    n > m.
+Proof.
+  induction t; intros m Hgt Hsucc; simpl in *; try discriminate.
+  inversion Hgt; subst.
+  destruct t1.
+  - (* successor is the root *)
+    injection Hsucc as <-. assumption.
+  - (* successor in left subtree *)
+    eapply IHt1; eauto.
+Qed.
+
+Lemma greater_delete :
+  forall n x t,
+    greater n t ->
+    greater n (delete x t).
+Proof.
+  induction t; intros; simpl.
+  - assumption.
+  - inversion H; subst.
+    destruct (n0 =? x) eqn:Heq.
+    + (* deleting root *)
+      destruct t1, t2; simpl; try assumption. 
+      destruct (successor (node t2_1 n2 t2_2)) eqn:Hsucc.
+      * (* successor found: n3 *)
+        destruct t2_1; simpl in *.
+        -- (* t2_1 = leaf, so successor is n2 *)
+           injection Hsucc as <-. simpl.
+           constructor.
+           ++ (* n > n2 *)
+              eapply greater_than_successor; eauto.
+           ++ (* greater n left *)
+              assumption.
+           ++ (* greater n t2_2 *)
+              inversion H6; subst. 
+              rewrite (Nat.eqb_refl n2). eauto.
+        -- (* t2_1 = node, successor from left subtree *)
+            admit.   
+        (* constructor.
+           ++ (* n > n3 *)
+              eapply greater_than_successor; eauto.
+           ++ (* greater n left *)
+              assumption.
+           ++ (* greater n (delete n3 right) *)
+              apply IHt2. assumption. *)
+      * (* no successor: impossible *)
+        eauto. admit.
+    + (* not deleting root *)
+      destruct (x <? n0) eqn:Hlt.
+      * constructor; try assumption; apply IHt1; assumption.
+      * constructor; try assumption; apply IHt2; assumption.
+Admitted.
+
+(* After deleting the successor from r, remaining elements are > successor *)
+Lemma successor_smaller_right_after_delete :
+  forall r m,
+    sorted r ->
+    successor r = Some m ->
+    smaller m (delete m r).
+Proof.
+  intros r m Hsort Hsucc.
+  (*
+  (* First: smaller m r from successor_all_right *)
+  apply smaller_delete_any.
+  eapply successor_all_right; eauto. *)
+  revert m Hsucc.
+  induction r; intros m Hsucc; simpl in *; try discriminate.
+  inversion Hsort; subst.
+  destruct r1.
+  - (* right subtree root is the successor, delete removes it and returns r2 *)
+    inversion Hsucc; subst. simpl. eauto. admit.
+  - (* successor comes from the left subtree *)
+    simpl in Hsucc. admit.
+Admitted.    
+    (* assert (m < v) as Hmv.
+    { (* successor from left is < v because all elements of left are < v *)
+      eapply successor_lt_root_left with (l:=r1) (r:=r2); eauto.
+    }
+    assert (v =? m = false) by (apply Nat.eqb_neq; lia).
+    assert (m <? v = true) by (apply Nat.ltb_lt; auto).
+    rewrite H0, H1. clear H0 H1.
+    constructor; try assumption.
+    + (* m < v *) exact Hmv.
+    + (* smaller m r2 via transitivity m < v and smaller v r2 *)
+      eapply smaller_lift_right; eauto. *)
+
+
+Lemma delete_sorted :
+  forall t x, sorted t -> sorted (delete x t).
+Proof.
+  induction t; intros x Hs; simpl.
+  - assumption.
+  - inversion Hs; subst.
+    destruct (n =? x) eqn:Heq.
+    + (* deleting root *)
+      destruct t1.
+      * (* no left subtree *)
+        destruct t2.
+        -- (* no right subtree: tree becomes leaf *) constructor.
+        -- (* one-child right: node leaf n0 t2_2 becomes t2 *) assumption.
+      * destruct t2.
+        -- (* one-child left *) assumption.
+        -- (* two children *)
+           destruct (successor (node t2_1 n1 t2_2)) eqn:Hsucc.
+           ++ (* successor found *)
+              simpl.
+              constructor.
+              ** (* greater n0 t1 *)
+                 eapply successor_greater_than_left; eauto.
+              ** (* smaller n0 (delete n0 right) *) 
+              rewrite Nat.eqb_eq in Heq; subst. 
+              rewrite <- (delete_unfold_node n2 n1 t2_1 t2_2).
+              eapply successor_smaller_right_after_delete; eauto.
+              ** (* sorted left *) assumption.
+              ** (* sorted right after delete *) eapply IHt2; assumption.
+           ++ (* No successor: impossible since right has at least root *)
+              simpl in Hsucc; eauto.
+    + (* not deleting root *)
+      destruct (x <? n) eqn:Hlt.
+      * (* delete in left *)
+        constructor; try assumption.
+        -- eapply greater_delete; eauto.
+        -- eapply IHt1; assumption.
+      * (* delete in right *)
+        constructor; try assumption.
+        -- eapply smaller_delete_any; eauto.
+        -- eapply IHt2; assumption.
+Qed.
+
+Lemma delete_correct :
+forall t x,
+    sorted t ->
+    elem_of x t = true -> 
+    (elem_of x (delete x t)) = false.
+Proof.
+  intros. 
+  induction t. simpl; intros.
+  - admit.
+  - inversion H. 
+Admitted.
+  
+
